wip

Veir/Passes/InstructionSelection/RISCV64.lean
@@ -46,7 +46,7 @@ def add (rewriter: PatternRewriter OpCode) (op: OperationPtr) :
   let (rewriter, rcastOp) ← rewriter.createOp (.builtin .unrealized_conversion_cast) #[RegisterType.mk] #[rhs]
       #[] #[] () (some $ .before op) sorry (by simp) (by simp) sorry
   /- Actual `riscv.add` -/
-  let (rewriter, addOp) ← rewriter.createOp (.riscv .add) #[RegisterType.mk] #[lcastOp.getResult 0, rcastOp.getResult 0]
+  let (rewriter, addOp) ← rewriter.createOp (.riscv .add) #[RegisterType.mk] #[rcastOp.getResult 0, lcastOp.getResult 0]
       #[] #[] () (some $ .before op) sorry (by simp) (by simp) sorry
   /- Cast back result for type consistency-/
   let (rewriter, castAddOp) ← rewriter.createOp (.builtin .unrealized_conversion_cast) #[type] #[addOp.getResult 0]
@@ -72,7 +72,7 @@ def and (rewriter: PatternRewriter OpCode) (op: OperationPtr) :
   let (rewriter, rcastOp) ← rewriter.createOp (.builtin .unrealized_conversion_cast) #[RegisterType.mk] #[rhs]
       #[] #[] () (some $ .before op) sorry (by simp) (by simp) sorry
   /- Actual `riscv.and` -/
-  let (rewriter, andOp) ← rewriter.createOp (.riscv .and) #[RegisterType.mk] #[lcastOp.getResult 0, rcastOp.getResult 0]
+  let (rewriter, andOp) ← rewriter.createOp (.riscv .and) #[RegisterType.mk] #[rcastOp.getResult 0, lcastOp.getResult 0]
       #[] #[] () (some $ .before op) sorry (by simp) (by simp) sorry
   /- Cast back result for type consistency-/
   let (rewriter, castAddOp) ← rewriter.createOp (.builtin .unrealized_conversion_cast) #[type] #[andOp.getResult 0]
@@ -98,7 +98,7 @@ def ashr (rewriter: PatternRewriter OpCode) (op: OperationPtr) :
   let (rewriter, rcastOp) ← rewriter.createOp (.builtin .unrealized_conversion_cast) #[RegisterType.mk] #[rhs]
       #[] #[] () (some $ .before op) sorry (by simp) (by simp) sorry
   /- Actual `riscv.sra` -/
-  let (rewriter, sraOp) ← rewriter.createOp (.riscv .sra) #[RegisterType.mk] #[lcastOp.getResult 0, rcastOp.getResult 0]
+  let (rewriter, sraOp) ← rewriter.createOp (.riscv .sra) #[RegisterType.mk] #[rcastOp.getResult 0, lcastOp.getResult 0]
       #[] #[] () (some $ .before op) sorry (by simp) (by simp) sorry
   /- Cast back result for type consistency-/
   let (rewriter, castSraOp) ← rewriter.createOp (.builtin .unrealized_conversion_cast) #[type] #[sraOp.getResult 0]
@@ -138,7 +138,7 @@ def icmp (rewriter: PatternRewriter OpCode) (op: OperationPtr) :
   let (rewriter, retOp) ← match property.predicate with
     | .eq =>
       /- llvm.icmp eq lhs rhs  -> riscv.sltiu (riscv.xor lhs rhs) 1 -/
-      let (rewriter, xorOp) ← rewriter.createOp (.riscv .xor) #[RegisterType.mk] #[lcastOp.getResult 0, rcastOp.getResult 0]
+      let (rewriter, xorOp) ← rewriter.createOp (.riscv .xor) #[RegisterType.mk] #[rcastOp.getResult 0, lcastOp.getResult 0]
         #[] #[] () (some $ .before op) sorry (by simp) (by simp) sorry
       let c1 := RISCVImmediateProperties.mk (IntegerAttr.mk 1 (IntegerType.mk 64))
       let (rewriter, retOp) ← rewriter.createOp (.riscv .sltiu) #[RegisterType.mk] #[xorOp.getResult 0]
@@ -146,7 +146,7 @@ def icmp (rewriter: PatternRewriter OpCode) (op: OperationPtr) :
       pure (rewriter, retOp)
     | .ne =>
       /- llvm.icmp ne lhs rhs  -> riscv.sltu 0 (riscv.xor lhs rhs) -/
-      let (rewriter, xorOp) ← rewriter.createOp (.riscv .xor) #[RegisterType.mk] #[lcastOp.getResult 0, rcastOp.getResult 0]
+      let (rewriter, xorOp) ← rewriter.createOp (.riscv .xor) #[RegisterType.mk] #[rcastOp.getResult 0, lcastOp.getResult 0]
         #[] #[] () (some $ .before op) sorry (by simp) (by simp) sorry
       let c0 := RISCVImmediateProperties.mk (IntegerAttr.mk 0 (IntegerType.mk 64))
       let (rewriter, liOp) ← rewriter.createOp (.riscv .li) #[RegisterType.mk] #[]
@@ -156,7 +156,7 @@ def icmp (rewriter: PatternRewriter OpCode) (op: OperationPtr) :
       pure (rewriter, retOp)
     | .slt =>
       /- llvm.icmp slt lhs rhs -> riscv.slt lhs rhs  -/
-      let (rewriter, retOp) ← rewriter.createOp (.riscv .slt) #[RegisterType.mk] #[lcastOp.getResult 0, rcastOp.getResult 0]
+      let (rewriter, retOp) ← rewriter.createOp (.riscv .slt) #[RegisterType.mk] #[rcastOp.getResult 0, lcastOp.getResult 0]
         #[] #[] () (some $ .before op) sorry (by simp) (by simp) sorry
       pure (rewriter, retOp)
     | .sle =>
@@ -174,7 +174,7 @@ def icmp (rewriter: PatternRewriter OpCode) (op: OperationPtr) :
       pure (rewriter, retOp)
     | .sge =>
       /- llvm.icmp sge lhs rhs -> riscv.xori (riscv_slt lhs rhs) 1 -/
-      let (rewriter, sltOp) ← rewriter.createOp (.riscv .slt) #[RegisterType.mk] #[lcastOp.getResult 0, rcastOp.getResult 0]
+      let (rewriter, sltOp) ← rewriter.createOp (.riscv .slt) #[RegisterType.mk] #[rcastOp.getResult 0, lcastOp.getResult 0]
         #[] #[] () (some $ .before op) sorry (by simp) (by simp) sorry
       let c1 := RISCVImmediateProperties.mk (IntegerAttr.mk 1 (IntegerType.mk 64))
       let (rewriter, retOp) ← rewriter.createOp (.riscv .xori) #[RegisterType.mk] #[sltOp.getResult 0]
@@ -182,7 +182,7 @@ def icmp (rewriter: PatternRewriter OpCode) (op: OperationPtr) :
       pure (rewriter, retOp)
     | .ult =>
       /- llvm.icmp ult lhs rhs -> riscv.sltu lhs rhs -/
-      let (rewriter, retOp) ← rewriter.createOp (.riscv .sltu) #[RegisterType.mk] #[lcastOp.getResult 0, rcastOp.getResult 0]
+      let (rewriter, retOp) ← rewriter.createOp (.riscv .sltu) #[RegisterType.mk] #[rcastOp.getResult 0, lcastOp.getResult 0]
         #[] #[] () (some $ .before op) sorry (by simp) (by simp) sorry
       pure (rewriter, retOp)
     | .ule =>
@@ -200,7 +200,7 @@ def icmp (rewriter: PatternRewriter OpCode) (op: OperationPtr) :
       pure (rewriter, retOp)
     | .uge =>
       /- llvm.icmp uge lhs rhs -> riscv.xori (riscv_sltu lhs rhs) 1 -/
-      let (rewriter, sltuOp) ← rewriter.createOp (.riscv .sltu) #[RegisterType.mk] #[lcastOp.getResult 0, rcastOp.getResult 0]
+      let (rewriter, sltuOp) ← rewriter.createOp (.riscv .sltu) #[RegisterType.mk] #[rcastOp.getResult 0, lcastOp.getResult 0]
         #[] #[] () (some $ .before op) sorry (by simp) (by simp) sorry
       let c1 := RISCVImmediateProperties.mk (IntegerAttr.mk 1 (IntegerType.mk 64))
       let (rewriter, retOp) ← rewriter.createOp (.riscv .xori) #[RegisterType.mk] #[sltuOp.getResult 0]
@@ -229,7 +229,7 @@ def or (rewriter: PatternRewriter OpCode) (op: OperationPtr) :
   let (rewriter, rcastOp) ← rewriter.createOp (.builtin .unrealized_conversion_cast) #[RegisterType.mk] #[rhs]
       #[] #[] () (some $ .before op) sorry (by simp) (by simp) sorry
   /- Actual `riscv.or` -/
-  let (rewriter, orOp) ← rewriter.createOp (.riscv .or) #[RegisterType.mk] #[lcastOp.getResult 0, rcastOp.getResult 0]
+  let (rewriter, orOp) ← rewriter.createOp (.riscv .or) #[RegisterType.mk] #[rcastOp.getResult 0, lcastOp.getResult 0]
       #[] #[] () (some $ .before op) sorry (by simp) (by simp) sorry
   /- Cast back result for type consistency-/
   let (rewriter, castOrOp) ← rewriter.createOp (.builtin .unrealized_conversion_cast) #[type] #[orOp.getResult 0]
@@ -255,7 +255,7 @@ def xor (rewriter: PatternRewriter OpCode) (op: OperationPtr) :
   let (rewriter, rcastOp) ← rewriter.createOp (.builtin .unrealized_conversion_cast) #[RegisterType.mk] #[rhs]
       #[] #[] () (some $ .before op) sorry (by simp) (by simp) sorry
   /- Actual `riscv.xor` -/
-  let (rewriter, xorOp) ← rewriter.createOp (.riscv .xor) #[RegisterType.mk] #[lcastOp.getResult 0, rcastOp.getResult 0]
+  let (rewriter, xorOp) ← rewriter.createOp (.riscv .xor) #[RegisterType.mk] #[rcastOp.getResult 0, lcastOp.getResult 0]
       #[] #[] () (some $ .before op) sorry (by simp) (by simp) sorry
   /- Cast back result for type consistency-/
   let (rewriter, castXorOp) ← rewriter.createOp (.builtin .unrealized_conversion_cast) #[type] #[xorOp.getResult 0]
@@ -281,7 +281,7 @@ def mul (rewriter: PatternRewriter OpCode) (op: OperationPtr) :
   let (rewriter, rcastOp) ← rewriter.createOp (.builtin .unrealized_conversion_cast) #[RegisterType.mk] #[rhs]
       #[] #[] () (some $ .before op) sorry (by simp) (by simp) sorry
   /- Actual `riscv.mul` -/
-  let (rewriter, mulOp) ← rewriter.createOp (.riscv .mul) #[RegisterType.mk] #[lcastOp.getResult 0, rcastOp.getResult 0]
+  let (rewriter, mulOp) ← rewriter.createOp (.riscv .mul) #[RegisterType.mk] #[rcastOp.getResult 0, lcastOp.getResult 0]
       #[] #[] () (some $ .before op) sorry (by simp) (by simp) sorry
   /- Cast back result for type consistency-/
   let (rewriter, castOp) ← rewriter.createOp (.builtin .unrealized_conversion_cast) #[type] #[mulOp.getResult 0]
@@ -307,7 +307,7 @@ def sdiv (rewriter: PatternRewriter OpCode) (op: OperationPtr) :
   let (rewriter, rcastOp) ← rewriter.createOp (.builtin .unrealized_conversion_cast) #[RegisterType.mk] #[rhs]
       #[] #[] () (some $ .before op) sorry (by simp) (by simp) sorry
   /- Actual `riscv.div` -/
-  let (rewriter, divOp) ← rewriter.createOp (.riscv .div) #[RegisterType.mk] #[lcastOp.getResult 0, rcastOp.getResult 0]
+  let (rewriter, divOp) ← rewriter.createOp (.riscv .div) #[RegisterType.mk] #[rcastOp.getResult 0, lcastOp.getResult 0]
       #[] #[] () (some $ .before op) sorry (by simp) (by simp) sorry
   /- Cast back result for type consistency-/
   let (rewriter, castOp) ← rewriter.createOp (.builtin .unrealized_conversion_cast) #[type] #[divOp.getResult 0]
@@ -333,7 +333,7 @@ def udiv (rewriter: PatternRewriter OpCode) (op: OperationPtr) :
   let (rewriter, rcastOp) ← rewriter.createOp (.builtin .unrealized_conversion_cast) #[RegisterType.mk] #[rhs]
       #[] #[] () (some $ .before op) sorry (by simp) (by simp) sorry
   /- Actual `riscv.div` -/
-  let (rewriter, divuOp) ← rewriter.createOp (.riscv .divu) #[RegisterType.mk] #[lcastOp.getResult 0, rcastOp.getResult 0]
+  let (rewriter, divuOp) ← rewriter.createOp (.riscv .divu) #[RegisterType.mk] #[rcastOp.getResult 0, lcastOp.getResult 0]
       #[] #[] () (some $ .before op) sorry (by simp) (by simp) sorry
   /- Cast back result for type consistency-/
   let (rewriter, castOp) ← rewriter.createOp (.builtin .unrealized_conversion_cast) #[type] #[divuOp.getResult 0]
@@ -359,7 +359,7 @@ def srem (rewriter: PatternRewriter OpCode) (op: OperationPtr) :
   let (rewriter, rcastOp) ← rewriter.createOp (.builtin .unrealized_conversion_cast) #[RegisterType.mk] #[rhs]
       #[] #[] () (some $ .before op) sorry (by simp) (by simp) sorry
   /- Actual `riscv.rem` -/
-  let (rewriter, remOp) ← rewriter.createOp (.riscv .rem) #[RegisterType.mk] #[lcastOp.getResult 0, rcastOp.getResult 0]
+  let (rewriter, remOp) ← rewriter.createOp (.riscv .rem) #[RegisterType.mk] #[rcastOp.getResult 0, lcastOp.getResult 0]
       #[] #[] () (some $ .before op) sorry (by simp) (by simp) sorry
   /- Cast back result for type consistency-/
   let (rewriter, castOp) ← rewriter.createOp (.builtin .unrealized_conversion_cast) #[type] #[remOp.getResult 0]
@@ -385,7 +385,7 @@ def urem (rewriter: PatternRewriter OpCode) (op: OperationPtr) :
   let (rewriter, rcastOp) ← rewriter.createOp (.builtin .unrealized_conversion_cast) #[RegisterType.mk] #[rhs]
       #[] #[] () (some $ .before op) sorry (by simp) (by simp) sorry
   /- Actual `riscv.remu` -/
-  let (rewriter, remuOp) ← rewriter.createOp (.riscv .remu) #[RegisterType.mk] #[lcastOp.getResult 0, rcastOp.getResult 0]
+  let (rewriter, remuOp) ← rewriter.createOp (.riscv .remu) #[RegisterType.mk] #[rcastOp.getResult 0, lcastOp.getResult 0]
       #[] #[] () (some $ .before op) sorry (by simp) (by simp) sorry
   /- Cast back result for type consistency-/
   let (rewriter, castOp) ← rewriter.createOp (.builtin .unrealized_conversion_cast) #[type] #[remuOp.getResult 0]
@@ -411,7 +411,7 @@ def sub (rewriter: PatternRewriter OpCode) (op: OperationPtr) :
   let (rewriter, rcastOp) ← rewriter.createOp (.builtin .unrealized_conversion_cast) #[RegisterType.mk] #[rhs]
       #[] #[] () (some $ .before op) sorry (by simp) (by simp) sorry
   /- Actual `riscv.remu` -/
-  let (rewriter, subOp) ← rewriter.createOp (.riscv .sub) #[RegisterType.mk] #[lcastOp.getResult 0, rcastOp.getResult 0]
+  let (rewriter, subOp) ← rewriter.createOp (.riscv .sub) #[RegisterType.mk] #[rcastOp.getResult 0, lcastOp.getResult 0]
       #[] #[] () (some $ .before op) sorry (by simp) (by simp) sorry
   /- Cast back result for type consistency-/
   let (rewriter, castOp) ← rewriter.createOp (.builtin .unrealized_conversion_cast) #[type] #[subOp.getResult 0]
@@ -564,7 +564,7 @@ def shl (rewriter: PatternRewriter OpCode) (op: OperationPtr) :
   let (rewriter, rcastOp) ← rewriter.createOp (.builtin .unrealized_conversion_cast) #[RegisterType.mk] #[rhs]
       #[] #[] () (some $ .before op) sorry (by simp) (by simp) sorry
   /- Actual `riscv.sll` -/
-  let (rewriter, mulOp) ← rewriter.createOp (.riscv .sll) #[RegisterType.mk] #[lcastOp.getResult 0, rcastOp.getResult 0]
+  let (rewriter, mulOp) ← rewriter.createOp (.riscv .sll) #[RegisterType.mk] #[rcastOp.getResult 0, lcastOp.getResult 0]
       #[] #[] () (some $ .before op) sorry (by simp) (by simp) sorry
   /- Cast back result for type consistency-/
   let (rewriter, castOp) ← rewriter.createOp (.builtin .unrealized_conversion_cast) #[type] #[mulOp.getResult 0]
@@ -590,7 +590,7 @@ def lshr (rewriter: PatternRewriter OpCode) (op: OperationPtr) :
   let (rewriter, rcastOp) ← rewriter.createOp (.builtin .unrealized_conversion_cast) #[RegisterType.mk] #[rhs]
       #[] #[] () (some $ .before op) sorry (by simp) (by simp) sorry
   /- Actual `riscv.srl` -/
-  let (rewriter, mulOp) ← rewriter.createOp (.riscv .srl) #[RegisterType.mk] #[lcastOp.getResult 0, rcastOp.getResult 0]
+  let (rewriter, mulOp) ← rewriter.createOp (.riscv .srl) #[RegisterType.mk] #[rcastOp.getResult 0, lcastOp.getResult 0]
       #[] #[] () (some $ .before op) sorry (by simp) (by simp) sorry
   /- Cast back result for type consistency-/
   let (rewriter, castOp) ← rewriter.createOp (.builtin .unrealized_conversion_cast) #[type] #[mulOp.getResult 0]
