Veir/Passes/InstructionSelection/Proofs.lean
@@ -1,5 +1,10 @@
 import Veir.Data.RISCV.Reg.Basic
+import Veir.Data.RISCV.Reg.Lemmas
+import Veir.Data.RISCV.Reg.Simp
 import Veir.Data.LLVM.Int.Basic
+import Veir.Data.LLVM.Int.Bitblast
+import Veir.Data.LLVM.Int.Simp
+import Veir.Data.LLVM.Int.Simp
 import Veir.Data.Casting
 import Veir.Data.Refinement
 import Std.Tactic.BVDecide
@@ -11,6 +16,26 @@ import Std.Tactic.BVDecide
 
 namespace Veir.Data.RISCV
 
+@[reg_toBitVec, grind =]
+theorem helper1 {r : RISCV.Reg} :
+    RISCV.Reg.toInt r 64 = (.val r.val) := by
+  simp [RISCV.Reg.toInt]
+
+@[llvm_toBitVec, grind =]
+theorem helper2 {x : LLVM.Int w} :
+    (LLVM.Int.toReg x).val = if h : x.isPoison then 0#64 else x.getValue.zeroExtend 64 := by
+  cases x <;> simp [LLVM.Int.toReg, llvm_toBitVec, LLVM.Int.getValue]
+
+@[reg_toBitVec, grind =]
+theorem helper3 {r : RISCV.Reg} :
+    (RISCV.Reg.toInt r w).isPoison = false := by
+  simp [RISCV.Reg.toInt, LLVM.Int.isPoison]
+
+@[reg_toBitVec, grind =]
+theorem helper4 {r : RISCV.Reg} :
+    (RISCV.Reg.toInt r w).getValue = r.val.zeroExtend w := by
+  simp [llvm_toBitVec, reg_toBitVec, RISCV.Reg.toInt]
+
 /--
   Prove the correctness of the `constant` lowering pattern.
 
@@ -18,23 +43,45 @@ namespace Veir.Data.RISCV
   are always concrete in the interpreter.
 -/
 theorem constant_refinement:
-    isRefinedBy (LLVM.Int.constant 64 v) (RISCV.Reg.toInt (Data.RISCV.li (BitVec.ofInt 64 v)) 64) := by
-  simp [isRefinedBy, Data.LLVM.Int.constant, Data.RISCV.li, RISCV.Reg.toInt]
+    (LLVM.Int.constant 64 v) ⊒ (RISCV.Reg.toInt (Data.RISCV.li (BitVec.ofInt 64 v)) 64) := by
+  simp [llvm_toBitVec, reg_toBitVec]
 
 /--
   Prove the correctness of the `add` lowering pattern.
 -/
 theorem add_refinement:
-    isRefinedBy (Data.LLVM.Int.add x y) (RISCV.Reg.toInt (Data.RISCV.add (LLVM.Int.toReg x) (LLVM.Int.toReg y)) 64) := by
-  simp only [isRefinedBy, Data.LLVM.Int.add, Bool.false_eq_true, false_and, ↓reduceIte,
-    pure_bind, RISCV.Reg.toInt, Data.RISCV.add, LLVM.Int.toReg, BitVec.truncate_eq_setWidth,
-    BitVec.setWidth_eq]
-  split
-  · split
-    · split
-      <;> bv_decide
-    · split
-      · bv_decide
-      · simp only [Id.run, Data.LLVM.Int.val.injEq] at *
-        bv_decide
-  · bv_decide
+    (Data.LLVM.Int.add x y) ⊒ (RISCV.Reg.toInt (Data.RISCV.add (LLVM.Int.toReg x) (LLVM.Int.toReg y)) 64) := by
+  simp [llvm_toBitVec, reg_toBitVec]
+  simp only [LLVM.Int.getValue_eq_getValueD]
+  bv_decide
+
+/--
+  Prove the correctness of the `and` lowering pattern.
+-/
+theorem and_refinement:
+    (Data.LLVM.Int.and x y) ⊒ (RISCV.Reg.toInt (Data.RISCV.and (LLVM.Int.toReg x) (LLVM.Int.toReg y)) 64) := by
+  simp [llvm_toBitVec, reg_toBitVec]
+  simp only [LLVM.Int.getValue_eq_getValueD]
+  bv_decide
+
+/--
+  Prove the correctness of the `ashr` lowering pattern.
+-/
+theorem ashr_refinement:
+    (Data.LLVM.Int.ashr x y) ⊒ (RISCV.Reg.toInt (Data.RISCV.sra (LLVM.Int.toReg y) (LLVM.Int.toReg x)) 64) := by
+  simp [llvm_toBitVec, reg_toBitVec]
+  simp only [LLVM.Int.getValue_eq_getValueD]
+  intros h1 h2
+  rw [Nat.mod_eq_of_lt (by
+      cases y <;> simp [h1, LLVM.Int.getValueD] at *;
+      exact Nat.lt_of_succ_le h2)]
+
+/--
+  Prove the correctness of the `icmp` lowering pattern with `eq`.
+-/
+theorem icmp_refinement:
+    (Data.LLVM.Int.icmp x y LLVM.IntPred.eq) ⊒
+      (RISCV.Reg.toInt (Data.RISCV.sltiu 1#12 (Data.RISCV.xor (LLVM.Int.toReg y) (LLVM.Int.toReg x))) 1) := by
+  simp [llvm_toBitVec, reg_toBitVec]
+
+  sorry
